Blocked: trying to simplify model for the proof

io/Proof.Model.fst
@@ -1,5 +1,6 @@
 module Proof.Model
 
+open FStar.List.Tot
 open FStar.Calc
 open FStar.Tactics
 
@@ -33,8 +34,8 @@ noeq type compiler = {
 
   compile_prog  : (#i:interface) -> (#pi:monitorable_prop) ->
                   prog_s i pi -> Tot (prog_t i);
-  compile_whole : (#i:interface) -> (#pi:monitorable_prop) ->
-                  whole_s i pi -> Tot (whole_t i);
+//  compile_whole : (#i:interface) -> (#pi:monitorable_prop) ->
+//                  whole_s i pi -> Tot (whole_t i);
 }
 
 noeq type interface = {
@@ -47,25 +48,13 @@ noeq type interface = {
   ret : Type;
 }
 
-(** Having a pre-condition for the context is not necessary,
-because the context can not use it. If we set a pre-condition
-for the context, the pre-condition is more of a promise that the
-partial-program has to fulfil. **)
+(** The whole program does not need a pre-condition. 
 
-(** For the context to have a post-condition, it makes sense only
-in one of the following cases:
-* a post-condition about the trace would be verrified after the
-  computation is over. Therefore, if the post-condition fails,
-  then it means the bad behavior already happened.
-* if the post-condition is only about the returned result, then
-  the post-condition could be written as a refinement on the type
-  of the result.
-* the only case in which it makes sense, is if the returned value
-  is a file descriptor and the post-condition looks like:
-  "the returned file_descriptor is open" **)
+Also, a post-condition would be useless since the system/
+environment can not use it. **)
 
 val whole_pre' : unit -> trace -> bool
-let whole_pre' _ _ = true
+let whole_pre' _ h = true 
 
 val whole_pre : unit -> trace -> Type0
 let whole_pre x h = whole_pre' x h
@@ -77,31 +66,43 @@ type whole_s (i:interface) (pi:monitorable_prop) =
   x:unit -> IIO i.ret pi (whole_pre x) (fun _ _ _ -> True)
 type whole_t (i:interface) = unit -> MIIO (maybe i.ret)
 
-(** the lift from "MIO to MIIO" for the context should happen
-during linking. It is improper to say "should happen", because
-the lift represents the assumptions: "the context uses
-only the IO library which comes with instrumentation".
- **)
+(** Having a pre-condition for the context is not necessary,
+because the context would not know about it. 
+If we set a pre-condition for the context, the pre-condition 
+is more of a promise that the partial-program has to fulfil.
+
+We make the following remarks about a context's post-condition:
+* If the post-condition is only about the returned result, then
+  the post-condition should be written as a refinement on the type
+  of the result.
+* At runtime, the post-condition is verified after the execution of
+  the context is over. Therefore, a safety property stated
+  in the post-condition would lose its 'safety' when checked at runtime,
+  because unsafe behavior could happen before the check happens.
+* a post-condition is needed. e.g.:
+  if the returned value is a file descriptor and the 
+  post-condition guarantees: "the returned file descriptor is open".
+**)
+
 let tpre : (i:interface) -> (i.ctx_arg -> trace -> bool) = fun i x h -> true
 type ctx_t (i:interface) = i.ctx_arg -> MIO i.ctx_ret
+(** The ctx_s stands for the instrumented context, therefore the
+    output type is different compared to ctx_t.
+    ctx_t has the output type `i.ctx_ret`, but ctx_s has `maybe i.ctx_ret`.
+    This is needed to accomodate the possibility of failure during 
+    instrumentation when a contract is violated. **)
 type ctx_s (i:interface) (pi:monitorable_prop) =
   (x:i.ctx_arg) -> IIO (maybe i.ctx_ret) pi (fun h -> tpre i x h) (i.ctx_post x)
 
+(** The partial program does not need a pre- or a post-condition because
+    it is the starting point of the execution in this model. **)
 type prog_s (i:interface) (pi:monitorable_prop) =
   ctx_s i pi -> IIO i.ret pi (fun _ -> True) (fun _ _ _ -> True)
+(** prog_t can not fail since it is statically verified. The instrumentation
+    of the context may return an error, but the partial program should treat
+    that error **)
 type prog_t (i:interface) (pi:monitorable_prop) =
-  ctx_s i pi -> MIIO (maybe i.ret)
-
-// let _ctx_p_types
-//   (i  : interface)
-//   (pi : monitorable_prop)
-//   (cp : ctx_p i pi)
-//   (x  : i.ctx_arg) :
-//   IIO i.ctx_ret pi (fun _ -> True) (fun _ _ _ -> True) =
-//   let r : i.ctx_ret_ci.itype = cp (export x) in
-//   match import r with
-//   | Some r -> r
-//   | None -> IIO.Effect.throw Contract_failure
+  ctx_s i pi -> MIIO i.ret
 
 let extract_local_trace (h:trace) (pi:monitorable_prop) :
   IIO trace pi
@@ -121,7 +122,7 @@ let extract_local_trace (h:trace) (pi:monitorable_prop) :
   assert (h' == apply_changes h (List.rev lt));
   List.rev lt
 
-(** CA: The body of this function was inlined in _import_IIO but the block
+(** CA: The body of this function was inlined in `instrument` but the block
 if-then-else added some extra weird goals which did not make sense,
 therefore a fast fix was extracting the block in a different function. **)
 let enforce_post
@@ -137,9 +138,9 @@ let enforce_post
     let b = check4 #t1 #trace #(maybe t2) #trace #post x h r lt in
     (b ==>  p r []) /\
     (~b ==>  p (Inr Contract_failure) [])) =
-  (if check4 #t1 #trace #(maybe t2) #trace #post x h r lt
+  if check4 #t1 #trace #(maybe t2) #trace #post x h r lt
   then r
-  else (Inr Contract_failure))
+  else (Inr Contract_failure)
 
 let instrument
   (i  : interface)
@@ -155,16 +156,36 @@ let instrument
     let lt : trace = extract_local_trace h pi in
     enforce_post #i.ctx_arg #i.ctx_ret i.ctx_post #i.ctx_post_c x h r lt
 
+(**
+  Context: During compilation, p is wrapped in a new function
+  that first does a runtime check. The runtime check verifies if the 
+  history respects pi. Since the partial program is our starting
+  point, the history is always empty, and the result of the runtime 
+  check is always true.
+
+  TODO: I don't know how to state that the history is always empty.
+**)
+
+(** Blocked: the assumption simplifies the compilation function, but
+I don't see how we can get rid of it. In the end, it can not be guaranteed
+that when the partial program starts, the history is empty. **)
+let compile_prog'
+  (#i  : interface)
+  (#pi : monitorable_prop)
+  (p  : prog_s i pi) 
+  (c : ctx_s i pi) :
+  MIIO i.ret by (iio_tactic ()) = 
+  assume (get_trace () == []);
+  p c
+
 let compile_prog
   (#i  : interface)
   (#pi : monitorable_prop)
   (p  : prog_s i pi) :
   Tot (prog_t i pi) =
-  _IIOwp_as_MIIO
-    (fun _ -> iio_pre pi)
-    (fun _ h r lt -> iio_post pi h r lt)
-    p
+      compile_prog' p
 
+(**
 let compile_whole
   (#i  : interface)
   (#pi : monitorable_prop)
@@ -173,8 +194,13 @@ let compile_whole
   _IIOwp_as_MIIO
     (fun _ -> iio_pre pi)
     (fun _ h r lt -> iio_post pi h r lt)
-    w
+    w**)
 
+(** the lift from "MIO to MIIO" for the context should happen
+during linking. It is improper to say "should happen", because
+the lift represents the assumptions: "the context uses
+only the IO library which comes with instrumentation".
+ **)
 val link_s  : (#i:interface) -> (#pi:monitorable_prop) -> ctx_s i pi ->
               prog_s i pi -> Tot (whole_s i pi)
 let link_s = (fun #i #pi c p -> (fun _ -> p c))
@@ -208,20 +234,87 @@ open FStar.WellFounded
   The lemma guarantees that computation p after being compiled
   still respects pi.
 
-  Context: During compilation, p is wrapped in a new function
-  that first does a runtime check. The final step of the
-  compilation is to change the effect from IIO, to MIIO and
-  remove the pre- and post-condition.
-
   Proof: The compilation process preserves the effect IIO and the
   pre- and post-condition until the last step, when there is a
   cast to MIIO, which does not influence the behavior of
   computation p.
+  
+  Just a note here about the Beh function. We did not know how to
+  define it when silent steps were involved. For io we had a Beh
+  function, but for io+exn, not. That's why we try to do the proof
+  using only the interpretation, because during the process of 
+  compilation, not much is changed. 
 **)
 
   // IIOwp (maybe 'b) (fun h p ->
   //   (~(pre x h) ==> p (Inr Contract_failure) []) /\
   //   (pre x h ==> (forall r lt. post x h r lt ==> p (Inl r) lt)))
+
+let interp = iio_interpretation
+
+let lemma_secure_prog_compilation
+  (#i  : interface)
+  (#pi : monitorable_prop)
+  (ps  : prog_s i pi)
+  (cs : ctx_s i pi) : 
+  IIOwp (maybe i.ret) (fun h p -> 
+    (~(iio_pre pi h) ==> p (Inr (Contract_failure)) []) /\
+      (iio_pre pi h ==>
+        (forall r lt. iio_post pi h r lt ==> p (Inl r) lt))) =
+    let pt = _IIOwp_as_IIO (fun _ h -> iio_pre pi h) (fun _ h r lt -> iio_post pi h r lt) ps in
+    let wt = (**IIOwp.**)reify (pt cs) [] (fun r lt -> 
+	    (~(iio_pre pi []) ==> r == (Inr Contract_failure) /\ lt == []) /\
+	    (iio_pre pi [] ==> iio_post pi [] r lt)) in
+     (** because (pt c) is in MIIO, we lose that it respects the interpretation **)
+    assert (interp wt [] (fun r lt -> 
+	    (~(iio_pre pi []) ==> r == (Inr Contract_failure) /\ lt == []) /\
+	    (iio_pre pi [] ==> iio_post pi [] r lt)));
+	    (**
+    let pt' : ctx_s i pi -> MIIO (maybe i.ret) = pt in
+    let wt' = (**MIIO.**)reify (pt' cs) [] (fun r lt -> True) in
+    assume (interp wt' [] (fun r lt -> 
+	    (~(iio_pre pi []) ==> r == (Inr Contract_failure) /\ lt == []) /\
+	    (iio_pre pi [] ==> iio_post pi [] r lt)));
+
+    let pt'' = compile_prog ps in
+    (** this two are not equal because one is in IIOwp and the other in MIIO **)
+(**    assert ((pt <: ctx_s i pi -> MIIO (maybe i.ret)) == pt') by (
+           norm [delta_only[`%compile_prog;`%_IIOwp_as_MIIO]];
+	   norm [iota]);**)**)
+	 _ by (dump "h");
+	 pt cs
+  
+     
+
+let lemma_secure_prog_compilation
+  (#i  : interface)
+  (#pi : monitorable_prop)
+  (p  : prog_s i pi)
+  (c : ctx_s i pi) :
+     Lemma (
+     	let ws = (**IIO.**)reify (p c) [] (fun r lt -> iio_post pi [] r lt) in
+     	interp ws [] (fun r lt -> iio_post pi [] r lt) ==> (
+	let pt = compile_prog p in
+	let wt = (**MIIO.**)reify (pt c) [] (fun r lt -> True) in
+	(** the problem is that because (pt c) is in MIIO, we lose the fact that it respects
+	    the interpretation **)
+	interp wt [] (fun r lt -> 
+	    (~(iio_pre pi []) ==> r == (Inr Contract_failure) /\ lt == []) /\
+	    (iio_pre pi [] ==> iio_post pi [] r lt))
+     )) =
+     	let pt = compile_prog p in
+	(** p is not equal with pt because of the following:
+	    1. pt adds a runtime checks that calls get_trace (). we are intersted in this 
+	       equality when the history is empty, therefore we should add a precondition
+	       stating that
+	    2. the output type of p is (t), but the output type for pt is (maybe t).
+	**)
+	assert (p == pt) by (
+           norm [delta_only[`%compile_prog;`%_IIOwp_as_MIIO;`%_IIOwp_as_IIO]];
+           norm [iota];
+	   dump "h");
+	()
+
 
 let lemma_secure_prog_compilation
   (#i  : interface)
